src/localdrf/LocalDRF_Config.v
@@ -1,0 +1,35 @@
+Require Import RelationClasses.
+
+From Paco Require Import paco.
+From sflib Require Import sflib.
+
+From PromisingLib Require Import Axioms.
+From PromisingLib Require Import Basic.
+From PromisingLib Require Import DataStructure.
+From PromisingLib Require Import Language.
+From PromisingLib Require Import Loc.
+Require Import Time.
+Require Import Event.
+Require Import View.
+Require Import Cell.
+Require Import Memory.
+Require Import MemoryFacts.
+Require Import TView.
+Require Import Local.
+Require Import Thread.
+Require Import Configuration.
+Require Import Progress.
+Require Import Behavior.
+Require Import Cover.
+Require Import Pred.
+Require Import Trace.
+Require Import JoinedView.
+
+Require Import MemoryProps.
+Require Import OrderedTimes.
+
+Require Import LocalDRFDef.
+Require Import LocalDRF_PF.
+Require Import CapMap.
+
+Set Implicit Arguments.
