src/localdrf/TimeTraced.v
@@ -1,0 +1,192 @@
+Require Import RelationClasses.
+
+From Paco Require Import paco.
+From sflib Require Import sflib.
+
+From PromisingLib Require Import Axioms.
+From PromisingLib Require Import Basic.
+From PromisingLib Require Import DataStructure.
+From PromisingLib Require Import Language.
+From PromisingLib Require Import Loc.
+Require Import Time.
+Require Import Event.
+Require Import View.
+Require Import Cell.
+Require Import Memory.
+Require Import MemoryFacts.
+Require Import TView.
+Require Import Local.
+Require Import Thread.
+Require Import Configuration.
+Require Import Progress.
+Require Import Behavior.
+
+Require Import Pred.
+Require Import Trace.
+Require Import OrderedTimes.
+Require Import PFConsistentStrong.
+
+Set Implicit Arguments.
+
+
+Inductive times_configuration_step (times: Loc.t -> Time.t -> Prop)
+  : forall (e:MachineEvent.t) (tid:Ident.t) (c1 c2:Configuration.t), Prop :=
+| times_step_intro
+    lang tr e tr' pf tid c1 st1 lc1 e2 st3 lc3 sc3 memory3
+    (TID: IdentMap.find tid c1.(Configuration.threads) = Some (existT _ lang st1, lc1))
+    (STEPS: Trace.steps tr' (Thread.mk _ st1 lc1 c1.(Configuration.sc) c1.(Configuration.memory)) e2)
+    (SILENT: List.Forall (fun the => ThreadEvent.get_machine_event (snd the) = MachineEvent.silent) tr')
+    (STEP: Thread.step pf e e2 (Thread.mk _ st3 lc3 sc3 memory3))
+    (TR: tr = tr'++[(e2, e)])
+    (CONSISTENT: forall (EVENT: e <> ThreadEvent.failure),
+        exists times_cert tr_cert,
+          (<<CONSISTENT: pf_consistent_super_strong
+                           (Thread.mk _ st3 lc3 sc3 memory3)
+                           times_cert
+                           tr_cert times>>))
+    (TIMES: List.Forall (fun thte => wf_time_evt times (snd thte)) tr)
+  :
+    times_configuration_step
+      times (ThreadEvent.get_machine_event e) tid c1 (Configuration.mk (IdentMap.add tid (existT _ _ st3, lc3) c1.(Configuration.threads)) sc3 memory3)
+.
+
+Lemma times_configuration_step_traced_step times e tid c1 c2
+      (STEP: times_configuration_step times e tid c1 c2)
+      (WF: Configuration.wf c1)
+  :
+    exists lang (tr: Trace.t lang),
+      (<<STEP: Trace.configuration_step tr e tid c1 c2>>).
+Proof.
+  inv STEP. esplits. econs; eauto.
+  i. exploit CONSISTENT; eauto. i. des.
+  dup WF. inv WF. exploit Trace.steps_future; eauto.
+  { ss. eapply WF1; eauto. } i. des. ss.
+  hexploit Trace.steps_future; eauto.
+  { eapply WF0; eauto. } i. des. ss.
+  hexploit Thread.step_future; eauto. i. des. ss.
+  eapply pf_consistent_super_strong_consistent; eauto.
+Qed.
+
+Lemma times_configuration_step_future
+      times e tid c1 c2
+      (STEP: times_configuration_step times e tid c1 c2)
+      (WF1: Configuration.wf c1):
+  (<<WF2: Configuration.wf c2>>) /\
+  (<<SC_FUTURE: TimeMap.le c1.(Configuration.sc) c2.(Configuration.sc)>>) /\
+  (<<MEM_FUTURE: Memory.future c1.(Configuration.memory) c2.(Configuration.memory)>>).
+Proof.
+  eapply times_configuration_step_traced_step in STEP; eauto. des.
+  eapply Trace.configuration_step_future; eauto.
+Qed.
+
+Lemma times_configuration_step_mon times0 times1
+      (LE: times0 <2= times1)
+  :
+    times_configuration_step times0 <4= times_configuration_step times1.
+Proof.
+  i. inv PR. econs; eauto.
+  { i. exploit CONSISTENT; eauto. i. des. esplits; eauto.
+    eapply pf_consistent_super_strong_mon; eauto. }
+  { eapply List.Forall_impl; eauto. i. eapply wf_time_evt_mon; eauto. }
+Qed.
+
+Lemma event_times_list_exists
+      e
+  :
+    exists (times: Loc.t -> list Time.t),
+      (<<EVT: wf_time_evt (fun loc ts => List.In ts (times loc)) e >>).
+Proof.
+  destruct e; ss; try by (exists (fun _ => []); splits; auto).
+  { exists (fun loc' => if Loc.eq_dec loc' loc then [from; to] else []).
+    des_ifs; ss; auto. }
+  { exists (fun loc' => if Loc.eq_dec loc' loc then [from; to] else []).
+    des_ifs; ss; auto. }
+  { exists (fun loc' => if Loc.eq_dec loc' loc then [tsr; tsw] else []).
+    des_ifs; ss; auto. }
+Qed.
+
+Lemma trace_fin_events lang (tr: Trace.t lang)
+  :
+    exists (times: Loc.t -> list Time.t),
+      (<<TIMES: List.Forall (fun thte => wf_time_evt (fun loc ts => List.In ts (times loc)) (snd thte)) tr>>).
+Proof.
+  induction tr.
+  { exists (fun _ => []). ss. }
+  { des. hexploit (event_times_list_exists (snd a)). i. des.
+    exists (fun loc => times loc ++ times0 loc). econs.
+    { eapply wf_time_evt_mon; eauto. i. ss.
+      eapply List.in_or_app; auto. }
+    { eapply List.Forall_impl; eauto. i. ss.
+      eapply wf_time_evt_mon; eauto. i. ss.
+      eapply List.in_or_app; auto. }
+  }
+Qed.
+
+Lemma times_configuration_step_exists c0 c1 tid e
+      (STEP: Configuration.step e tid c0 c1)
+      (WF: Configuration.wf c0)
+  :
+    exists times,
+      (<<STEP: times_configuration_step times e tid c0 c1>>) /\
+      (<<WO: forall loc, well_ordered (times loc)>>).
+Proof.
+  eapply Trace.step_configuration_step in STEP. des.
+  hexploit (trace_fin_events tr). i. des. inv STEP0.
+  eapply inj_pair2 in H1. subst. destruct (classic (e0 = ThreadEvent.failure)).
+  { subst. exists (fun loc ts => List.In ts (times loc)). splits.
+    { econs; eauto. ss. }
+    { i. eapply finite_well_ordered. }
+  }
+  { hexploit CONSISTENT; ss.
+    dup WF. inv WF. exploit Trace.steps_future; eauto.
+    { ss. eapply WF1; eauto. } i. des. ss.
+    hexploit Thread.step_future; eauto. i. des. ss.
+    eapply consistent_pf_consistent_super_strong in H0; eauto.
+    des. exists (certimes \2/ (fun loc ts => List.In ts (times loc))). splits.
+    { econs; eauto.
+      { i. esplits. eapply pf_consistent_super_strong_mon; eauto. }
+      { eapply List.Forall_impl; try apply TIMES.
+        i. ss. eapply wf_time_evt_mon; try apply H0. i. ss. auto. }
+    }
+    { i. eapply join_well_ordered; eauto. eapply finite_well_ordered. }
+  }
+Qed.
+
+Lemma times_configuration_step_same_behaviors c beh
+      (WF: Configuration.wf c)
+      (BEH: behaviors Configuration.step c beh)
+  :
+    exists times,
+      (<<BEH: behaviors (times_configuration_step times) c beh>>) /\
+      (<<WO: forall loc, well_ordered (times loc)>>).
+Proof.
+  ginduction BEH.
+  { i. exists bot2. splits.
+    { econs 1; eauto. }
+    { i. eapply empty_well_ordered. }
+  }
+  { i. exploit IHBEH.
+    { eapply Configuration.step_future; eauto. } i. des.
+    exploit times_configuration_step_exists; eauto. i. des.
+    exists (times \2/ times0). splits.
+    { econs 2; eauto.
+      { eapply times_configuration_step_mon; eauto. }
+      { eapply le_step_behavior_improve; try apply BEH0.
+        eapply times_configuration_step_mon. i. auto. }
+    }
+    { i. eapply join_well_ordered; eauto. }
+  }
+  { i. exploit times_configuration_step_exists; eauto. i. des.
+    exists times. splits; eauto. econs 3; eauto. }
+  { i. exploit IHBEH.
+    { eapply Configuration.step_future; eauto. } i. des.
+    exploit times_configuration_step_exists; eauto. i. des.
+    exists (times \2/ times0). splits.
+    { econs 4; eauto.
+      { eapply times_configuration_step_mon; eauto. }
+      { eapply le_step_behavior_improve; try apply BEH0.
+        eapply times_configuration_step_mon. i. auto. }
+    }
+    { i. eapply join_well_ordered; eauto. }
+  }
+Qed.
