src/prop/Trace.v
@@ -104,14 +104,52 @@ Module Trace.
   | step_intro
       lang tr e tr' pf tid c1 st1 lc1 e2 st3 lc3 sc3 memory3
       (TID: IdentMap.find tid c1.(Configuration.threads) = Some (existT _ lang st1, lc1))
-      (STEPS: steps tr (Thread.mk _ st1 lc1 c1.(Configuration.sc) c1.(Configuration.memory)) e2)
-      (SILENT: List.Forall (fun the => ThreadEvent.get_machine_event (snd the) = MachineEvent.silent) tr)
+      (STEPS: steps tr' (Thread.mk _ st1 lc1 c1.(Configuration.sc) c1.(Configuration.memory)) e2)
+      (SILENT: List.Forall (fun the => ThreadEvent.get_machine_event (snd the) = MachineEvent.silent) tr')
       (STEP: Thread.step pf e e2 (Thread.mk _ st3 lc3 sc3 memory3))
-      (TR: tr' = tr++[(e2, e)])
+      (TR: tr = tr'++[(e2, e)])
       (CONSISTENT: forall (EVENT: e <> ThreadEvent.failure),
           Thread.consistent (Thread.mk _ st3 lc3 sc3 memory3))
     :
       configuration_step tr (ThreadEvent.get_machine_event e) tid c1 (Configuration.mk (IdentMap.add tid (existT _ _ st3, lc3) c1.(Configuration.threads)) sc3 memory3)
   .
+
+  Lemma configuration_step_step lang tr e tid c1 c2
+        (STEP: @configuration_step lang tr e tid c1 c2)
+    :
+      Configuration.step e tid c1 c2.
+  Proof.
+    inv STEP. destruct (classic (e0 = ThreadEvent.failure)).
+    { subst. econs 1; try apply STEP0; eauto.
+      eapply silent_steps_tau_steps; eauto. }
+    { econs 2; try apply STEP0; eauto.
+      eapply silent_steps_tau_steps; eauto. }
+  Qed.
+
+  Lemma step_configuration_step e tid c1 c2
+        (STEP: Configuration.step e tid c1 c2)
+    :
+      exists lang tr,
+        (<<STEP: @configuration_step lang tr e tid c1 c2>>).
+  Proof.
+    inv STEP.
+    { eapply tau_steps_silent_steps in STEPS. des.
+      replace MachineEvent.failure with (ThreadEvent.get_machine_event ThreadEvent.failure); auto.
+      esplits. econs; eauto. i. ss. }
+    { eapply tau_steps_silent_steps in STEPS. des.
+      esplits. econs; eauto. }
+  Qed.
+
+  Lemma configuration_step_future
+        lang (tr: t lang) e tid c1 c2
+        (STEP: configuration_step tr e tid c1 c2)
+        (WF1: Configuration.wf c1):
+    (<<WF2: Configuration.wf c2>>) /\
+    (<<SC_FUTURE: TimeMap.le c1.(Configuration.sc) c2.(Configuration.sc)>>) /\
+    (<<MEM_FUTURE: Memory.future c1.(Configuration.memory) c2.(Configuration.memory)>>).
+  Proof.
+    eapply configuration_step_step in STEP.
+    eapply Configuration.step_future; eauto.
+  Qed.
 
 End Trace.
